Ideal interop memcpy

src/arch/x64/interop/Memcpy.fst
@@ -23,54 +23,13 @@ open X64.Vale.Lemmas_i
 module TS = X64.Taint_Semantics_s
 module ME = X64.Memory_i_s
 module BS = X64.Bytes_Semantics_s
-#set-options "--z3rlimit 40"
+#set-options "--z3rlimit 60"
 
 open Vale_memcpy
 
-#set-options "--initial_fuel 5 --max_fuel 5 --initial_ifuel 2 --max_ifuel 2"
-// TODO: Prove these two lemmas if they are not proven automatically
-let win_implies_pre (h0:HS.mem) (dst:s8) (src:s8)  (stack_b:b8) : Lemma
-  (requires pre_cond h0 dst src /\ B.length stack_b == 24 /\ live h0 stack_b /\ buf_disjoint_from stack_b [dst;src])
-  (ensures (
-B.length stack_b == 24 /\ live h0 stack_b /\ buf_disjoint_from stack_b [dst;src] /\ (  let taint_func (x:b8) : GTot taint =
-    if StrongExcludedMiddle.strong_excluded_middle (x == dst) then Secret else
-    if StrongExcludedMiddle.strong_excluded_middle (x == src) then Secret else
-    Public in
-  let buffers = stack_b::dst::src::[] in
-  let (mem:mem) = {addrs = addrs; ptrs = buffers; hs = h0} in
-  let addr_dst = addrs dst in
-  let addr_src = addrs src in
-  let addr_stack:nat64 = addrs stack_b + 0 in
-  let regs = fun r -> begin match r with
-    | Rsp -> addr_stack
-    | Rcx -> addr_dst
-    | Rdx -> addr_src
-    | _ -> init_regs r end in
-  let xmms = init_xmms in
-  let s0 = {ok = true; regs = regs; xmms = xmms; flags = 0; mem = mem; memTaint = create_valid_memtaint mem buffers taint_func} in
-  length_t_eq (TBase TUInt64) stack_b;
-  length_t_eq (TBase TUInt64) dst;
-  length_t_eq (TBase TUInt64) src;
-  va_pre (va_code_memcpy true) s0 true stack_b dst src ))) =
-  length_t_eq (TBase TUInt64) stack_b;
-  length_t_eq (TBase TUInt64) dst;
-  length_t_eq (TBase TUInt64) src;
-  assert(B.disjoint stack_b dst);
-  assert(B.disjoint stack_b src);
-  ()
+#set-options "--initial_fuel 7 --max_fuel 7 --initial_ifuel 4 --max_ifuel 4"
 
-let win_implies_post (va_s0:va_state) (va_sM:va_state) (va_fM:va_fuel) (dst:s8) (src:s8)  (stack_b:b8) : Lemma
-  (requires pre_cond va_s0.mem.hs dst src /\ B.length stack_b == 24 /\ live va_s0.mem.hs stack_b /\ buf_disjoint_from stack_b [dst;src]/\
-    va_post (va_code_memcpy true) va_s0 va_sM va_fM true stack_b dst src )
-  (ensures post_cond va_s0.mem.hs va_sM.mem.hs dst src ) =
-  length_t_eq (TBase TUInt64) stack_b;
-  length_t_eq (TBase TUInt64) dst;
-  length_t_eq (TBase TUInt64) src;
-  ()
-
-val win_ghost_memcpy: dst:s8 -> src:s8 ->  stack_b:b8 -> (h0:HS.mem{pre_cond h0 dst src /\ B.length stack_b == 24 /\ live h0 stack_b /\ buf_disjoint_from stack_b [dst;src]}) -> GTot (h1:HS.mem{post_cond h0 h1 dst src })
-
-let win_ghost_memcpy dst src stack_b h0 =
+let create_initial_state w dst src stack_b (h0:HS.mem{pre_cond h0 dst src /\ B.length stack_b == 24 /\ live h0 stack_b /\ buf_disjoint_from stack_b [dst;src]}) : GTot TS.traceState =
   let taint_func (x:b8) : GTot taint =
     if StrongExcludedMiddle.strong_excluded_middle (x == dst) then Secret else
     if StrongExcludedMiddle.strong_excluded_middle (x == src) then Secret else
@@ -80,159 +39,89 @@ let win_ghost_memcpy dst src stack_b h0 =
   let addr_dst = addrs dst in
   let addr_src = addrs src in
   let addr_stack:nat64 = addrs stack_b + 0 in
-  let regs = fun r -> begin match r with
-    | Rsp -> addr_stack
-    | Rcx -> addr_dst
-    | Rdx -> addr_src
-    | _ -> init_regs r end in
-  let xmms = init_xmms in
-  let s0 = {ok = true; regs = regs; xmms = xmms; flags = 0; mem = mem; memTaint = create_valid_memtaint mem buffers taint_func} in
-  length_t_eq (TBase TUInt64) stack_b;
-  length_t_eq (TBase TUInt64) dst;
-  length_t_eq (TBase TUInt64) src;
-  win_implies_pre h0 dst src stack_b ;
-  let s1, f1 = va_lemma_memcpy (va_code_memcpy true) s0 true stack_b dst src  in
-  // Ensures that the Vale execution was correct
-  assert(s1.ok);
-  // Ensures that the callee_saved registers are correct
-  assert(s0.regs Rbx == s1.regs Rbx);
-  assert(s0.regs Rbp == s1.regs Rbp);
-  assert(s0.regs Rdi == s1.regs Rdi);
-  assert(s0.regs Rsi == s1.regs Rsi);
-  assert(s0.regs Rsp == s1.regs Rsp);
-  assert(s0.regs R12 == s1.regs R12);
-  assert(s0.regs R13 == s1.regs R13);
-  assert(s0.regs R14 == s1.regs R14);
-  assert(s0.regs R15 == s1.regs R15);
-  assert(s0.xmms 6 == s1.xmms 6);
-  assert(s0.xmms 7 == s1.xmms 7);
-  assert(s0.xmms 8 == s1.xmms 8);
-  assert(s0.xmms 9 == s1.xmms 9);
-  assert(s0.xmms 10 == s1.xmms 10);
-  assert(s0.xmms 11 == s1.xmms 11);
-  assert(s0.xmms 12 == s1.xmms 12);
-  assert(s0.xmms 13 == s1.xmms 13);
-  assert(s0.xmms 14 == s1.xmms 14);
-  assert(s0.xmms 15 == s1.xmms 15);
-  // Ensures that va_code_memcpy is actually Vale code, and that s1 is the result of executing this code
-  assert (va_ensure_total (va_code_memcpy true) s0 s1 f1);
-  win_implies_post s0 s1 f1 dst src stack_b ;
-  s1.mem.hs
-
-// TODO: Prove these two lemmas if they are not proven automatically
-let lin_implies_pre (h0:HS.mem) (dst:s8) (src:s8)  (stack_b:b8) : Lemma
-  (requires pre_cond h0 dst src /\ B.length stack_b == 24 /\ live h0 stack_b /\ buf_disjoint_from stack_b [dst;src])
-  (ensures (
-B.length stack_b == 24 /\ live h0 stack_b /\ buf_disjoint_from stack_b [dst;src] /\ (  let taint_func (x:b8) : GTot taint =
-    if StrongExcludedMiddle.strong_excluded_middle (x == dst) then Secret else
-    if StrongExcludedMiddle.strong_excluded_middle (x == src) then Secret else
-    Public in
-  let buffers = stack_b::dst::src::[] in
-  let (mem:mem) = {addrs = addrs; ptrs = buffers; hs = h0} in
-  let addr_dst = addrs dst in
-  let addr_src = addrs src in
-  let addr_stack:nat64 = addrs stack_b + 0 in
-  let regs = fun r -> begin match r with
-    | Rsp -> addr_stack
-    | Rdi -> addr_dst
-    | Rsi -> addr_src
-    | _ -> init_regs r end in
-  let xmms = init_xmms in
-  let s0 = {ok = true; regs = regs; xmms = xmms; flags = 0; mem = mem; memTaint = create_valid_memtaint mem buffers taint_func} in
-  length_t_eq (TBase TUInt64) stack_b;
-  length_t_eq (TBase TUInt64) dst;
-  length_t_eq (TBase TUInt64) src;
-  va_pre (va_code_memcpy false) s0 false stack_b dst src ))) =
-  length_t_eq (TBase TUInt64) stack_b;
-  length_t_eq (TBase TUInt64) dst;
-  length_t_eq (TBase TUInt64) src;
-  assert(B.disjoint stack_b dst);
-  assert(B.disjoint stack_b src);
-  ()
-
-let lin_implies_post (va_s0:va_state) (va_sM:va_state) (va_fM:va_fuel) (dst:s8) (src:s8)  (stack_b:b8) : Lemma
-  (requires pre_cond va_s0.mem.hs dst src /\ B.length stack_b == 24 /\ live va_s0.mem.hs stack_b /\ buf_disjoint_from stack_b [dst;src]/\
-    va_post (va_code_memcpy false) va_s0 va_sM va_fM false stack_b dst src )
-  (ensures post_cond va_s0.mem.hs va_sM.mem.hs dst src ) =
-  length_t_eq (TBase TUInt64) stack_b;
-  length_t_eq (TBase TUInt64) dst;
-  length_t_eq (TBase TUInt64) src;
-  ()
-
-let lin_calling_conv (s0:TS.traceState) (s1:TS.traceState) =
-  let s0_b= s0.TS.state.ME.state in
-  let s_b = s1.TS.state.ME.state in
-  // Ensures that the execution didn't crash
-  s_b.BS.ok /\
-  // Ensures that the callee_saved registers are correct
-  s0_b.BS.regs Rbx == s_b.BS.regs Rbx /\
-  s0_b.BS.regs Rbp == s_b.BS.regs Rbp /\
-  s0_b.BS.regs R12 == s_b.BS.regs R12 /\
-  s0_b.BS.regs R13 == s_b.BS.regs R13 /\
-  s0_b.BS.regs R14 == s_b.BS.regs R14 /\
-  s0_b.BS.regs R15 == s_b.BS.regs R15
-
-
-let create_initial_state dst src stack_b (h0:HS.mem{pre_cond h0 dst src /\ B.length stack_b == 24 /\ live h0 stack_b /\ buf_disjoint_from stack_b [dst;src]}) : GTot TS.traceState =
-  let taint_func (x:b8) : GTot taint =
-    if StrongExcludedMiddle.strong_excluded_middle (x == dst) then Secret else
-    if StrongExcludedMiddle.strong_excluded_middle (x == src) then Secret else
-    Public in
-  let buffers = stack_b::dst::src::[] in
-  let (mem:mem) = {addrs = addrs; ptrs = buffers; hs = h0} in
-  let addr_dst = addrs dst in
-  let addr_src = addrs src in
-  let addr_stack:nat64 = addrs stack_b + 0 in
-  let regs = fun r -> begin match r with
-    | Rsp -> addr_stack
-    | Rdi -> addr_dst
-    | Rsi -> addr_src
-    | _ -> init_regs r end in
+  let regs = if w then (
+    fun r -> begin match r with
+      | Rsp -> addr_stack
+      | Rcx -> addr_dst
+      | Rdx -> addr_src
+      | _ -> init_regs r end)
+  else (
+    fun r -> begin match r with
+      | Rsp -> addr_stack
+      | Rdi -> addr_dst
+      | Rsi -> addr_src
+      | _ -> init_regs r end)
+  in
   let xmms = init_xmms in
   let (s_b:BS.state) = {BS.ok = true; BS.regs = regs; BS.xmms = xmms; BS.flags = 0; BS.mem = Interop.down_mem mem.hs mem.addrs mem.ptrs} in
   let s0:X64.Memory_i_s.state = {ME.state = s_b; ME.mem = mem} in
   {TS.state = s0; TS.trace = []; TS.memTaint = create_valid_memtaint mem buffers taint_func}
 
-val lin_ghost_memcpy: dst:s8 -> src:s8 ->  stack_b:b8 -> (h0:HS.mem{pre_cond h0 dst src /\ B.length stack_b == 24 /\ live h0 stack_b /\ buf_disjoint_from stack_b [dst;src]}) -> GTot 
-  (s1:TS.traceState{post_cond h0 (s1.TS.state.ME.mem.hs) dst src /\ lin_calling_conv (create_initial_state dst src stack_b h0) s1})
-//(h1:HS.mem{post_cond h0 h1 dst src })
-
-val lemma_lin_ghost_memcpy:  dst:s8 -> src:s8 ->  stack_b:b8 -> (h0:HS.mem{pre_cond h0 dst src /\ B.length stack_b == 24 /\ live h0 stack_b /\ buf_disjoint_from stack_b [dst;src]}) ->
-  Ghost nat
-    (requires True)
-    (ensures (fun f1 ->
-      (let s0 = create_initial_state dst src stack_b h0 in
-       let s1 = TS.taint_eval_code (va_code_memcpy false) f1 s0 in
-       Some? s1 /\
-       post_cond h0 ((Some?.v s1).TS.state.ME.mem.hs) dst src /\
-       lin_calling_conv s0 (Some?.v s1))
-      )
-    )
-
-let lemma_lin_ghost_memcpy dst src stack_b h0 =
+let implies_pre (w:bool) (h0:HS.mem) (dst:s8) (src:s8)  (stack_b:b8) : Lemma
+  (requires pre_cond h0 dst src /\ B.length stack_b == 24 /\ live h0 stack_b /\ buf_disjoint_from stack_b [dst;src])
+  (ensures (
+  B.length stack_b == 24 /\ live h0 stack_b /\ buf_disjoint_from stack_b [dst;src] /\ (
+  let s0 = state_of_S (create_initial_state w dst src stack_b h0) in
   length_t_eq (TBase TUInt64) stack_b;
   length_t_eq (TBase TUInt64) dst;
   length_t_eq (TBase TUInt64) src;
-  lin_implies_pre h0 dst src stack_b ;
-  let s0 = create_initial_state dst src stack_b h0 in
-  let s_v, f_v = va_lemma_memcpy (va_code_memcpy false) (state_of_S s0) false stack_b dst src in  
-  lin_implies_post (state_of_S s0) s_v f_v dst src stack_b;
+  va_pre (va_code_memcpy w) s0 w stack_b dst src))) =
+  length_t_eq (TBase TUInt64) stack_b;
+  length_t_eq (TBase TUInt64) dst;
+  length_t_eq (TBase TUInt64) src;
+  assert(B.disjoint stack_b dst);
+  assert(B.disjoint stack_b src);
+  ()
+
+let implies_post (w:bool) (va_s0:va_state) (va_sM:va_state) (va_fM:va_fuel) (dst:s8) (src:s8)  (stack_b:b8) : Lemma
+  (requires pre_cond va_s0.mem.hs dst src /\ B.length stack_b == 24 /\ live va_s0.mem.hs stack_b /\ buf_disjoint_from stack_b [dst;src]/\
+    va_post (va_code_memcpy w) va_s0 va_sM va_fM w stack_b dst src )
+  (ensures post_cond va_s0.mem.hs va_sM.mem.hs dst src ) =
+  length_t_eq (TBase TUInt64) stack_b;
+  length_t_eq (TBase TUInt64) dst;
+  length_t_eq (TBase TUInt64) src;
+  ()
+
+val ghost_memcpy_aux: w:bool -> dst:s8 -> src:s8 ->  stack_b:b8 -> (h0:HS.mem{pre_cond h0 dst src /\ B.length stack_b == 24 /\ live h0 stack_b /\ buf_disjoint_from stack_b [dst;src]}) -> GTot 
+  (s1:TS.traceState{post_cond h0 (s1.TS.state.ME.mem.hs) dst src /\ calling_conventions w (create_initial_state w dst src stack_b h0) s1})
+
+val lemma_ghost_memcpy:  w:bool -> dst:s8 -> src:s8 ->  stack_b:b8 -> (h0:HS.mem{pre_cond h0 dst src /\ B.length stack_b == 24 /\ live h0 stack_b /\ buf_disjoint_from stack_b [dst;src]}) ->
+  Ghost nat
+    (requires True)
+    (ensures (fun f1 ->
+      (let s0 = create_initial_state w dst src stack_b h0 in
+       let s1 = TS.taint_eval_code (va_code_memcpy w) f1 s0 in
+       Some? s1 /\
+       post_cond h0 ((Some?.v s1).TS.state.ME.mem.hs) dst src /\
+       calling_conventions w s0 (Some?.v s1))
+      )
+    )
+
+let lemma_ghost_memcpy w dst src stack_b h0 =
+  length_t_eq (TBase TUInt64) stack_b;
+  length_t_eq (TBase TUInt64) dst;
+  length_t_eq (TBase TUInt64) src;
+  implies_pre w h0 dst src stack_b ;
+  let s0 = create_initial_state w dst src stack_b h0 in
+  let s_v, f_v = va_lemma_memcpy (va_code_memcpy w) (state_of_S s0) w stack_b dst src in  
+  implies_post w (state_of_S s0) s_v f_v dst src stack_b;
   f_v
   
 
-let lin_ghost_memcpy dst src stack_b h0 =
-  let s0 = create_initial_state dst src stack_b h0 in
-
-  let f1 = lemma_lin_ghost_memcpy dst src stack_b h0 in
-  let s1 = TS.taint_eval_code (va_code_memcpy false) f1 s0 in
+let ghost_memcpy_aux w dst src stack_b h0 =
+  let s0 = create_initial_state w dst src stack_b h0 in
+  let f1 = lemma_ghost_memcpy w dst src stack_b h0 in
+  let s1 = TS.taint_eval_code (va_code_memcpy w) f1 s0 in
   (Some?.v s1)
+
 
 val ghost_memcpy: dst:s8 -> src:s8 ->  stack_b:b8 -> (h0:HS.mem{pre_cond h0 dst src /\ B.length stack_b == 24 /\ live h0 stack_b /\ buf_disjoint_from stack_b [dst;src]}) -> GTot 
   (h1:HS.mem{post_cond h0 h1 dst src})
 
 let ghost_memcpy dst src stack_b h0 =
-  if win then win_ghost_memcpy dst src stack_b h0
-  else (lin_ghost_memcpy dst src stack_b h0).TS.state.ME.mem.hs
+  if win then (ghost_memcpy_aux true dst src stack_b h0).TS.state.ME.mem.hs
+  else (ghost_memcpy_aux false dst src stack_b h0).TS.state.ME.mem.hs
+
 
 let memcpy dst src  =
   push_frame();
